theory/JITPer_jump.thy
@@ -1,0 +1,34 @@
+theory JITPer_jump
+imports
+  Main
+  rBPFCommType rBPFSyntax rBPFSem
+  x64Syntax x64Semantics x64Assembler
+  JITPer_aux
+
+begin
+
+lemma ja_subgoal_rr_generic:
+  assumes a0:"bins = BPF_JA d" and
+       a1:"per_jit_ja (scast d) = Some (n, off, l_bin)" and
+       a3:"x64_decode 0 l_bin = Some (length l_bin, xins)" and
+       a4:"sbpf_step prog (SBPF_OK pc rs m) = (SBPF_OK pc' rs' m')" and
+       a5:"Next spc' reg' xm' = exec_instr xins sz spc reg xm" and
+       a6:"match_state (SBPF_OK pc rs m) (Next spc reg xm) " and
+       a7:"prog!(unat pc) = bins"
+  shows "match_state (SBPF_OK pc' rs' m') (Next spc' reg' xm') "
+proof -
+    have b0:"xins = Pjmp 0" 
+      using x64_encode_decode_consistency per_jit_ja_def a1 a3 list_in_list_prop
+    by (smt (verit, ccfv_SIG) Pair_inject map_option_eq_Some option.inject)
+    moreover have b1:"(\<forall> r. (rs r) = reg (bpf_to_x64_reg r))" using a6 spec match_state_def match_reg_def by simp
+    have b2:"\<forall> r. reg'(bpf_to_x64_reg r) = reg (bpf_to_x64_reg r)" using b0 a5 by (simp add: exec_instr_def)
+    have b3:"\<forall> r. (rs' r) = (rs r)" using a0 a4 a7 
+      by (metis (no_types, lifting) bpf_instruction.simps(375) sbpf_state.distinct(3) sbpf_state.inject(1) sbpf_step.simps(1))
+    have b4:"(\<forall> r. (rs' r) = reg' ((bpf_to_x64_reg r)))" using b1 b2 b3 by presburger
+    have b8:"match_stack reg' xm'" using a6 match_state_def a5 b0 by (simp add: exec_instr_def)
+    have b9:"match_mem m' xm'" using match_state_def a6 a5 b0 apply (simp add: exec_instr_def) 
+      using a4 mem_is_not_changed by blast
+    thus ?thesis using b4  match_state_def b8 b9 match_reg_def by fastforce
+  qed
+      
+end
